Fixed some integrity typos. Proving measurement part2 halfway.

AbstractPlatform/MeasurementProof.bpl
@@ -29,6 +29,14 @@ procedure {:inline 1} MeasurementEnclaveComputation(iter : int)
     var way     : cache_way_index_t;
     var i_eid   : tap_enclave_id_t;
     var is_invalid_id : bool;
+    var another_eid : tap_enclave_id_t;
+
+    // Determine another trace's eid, just for validation sync.
+    // Not elegant, but it's Z3-provable. Quite weird.
+    another_eid := cpu_enclave_id_1;    
+    assume (cpu_enclave_id_1 != cpu_enclave_id_2 && cpu_enclave_id == cpu_enclave_id_1) ==> (another_eid == cpu_enclave_id_2);
+    assume (cpu_enclave_id_1 != cpu_enclave_id_2 && cpu_enclave_id == cpu_enclave_id_2) ==> (another_eid == cpu_enclave_id_1);
+    assume (cpu_enclave_id_1 == cpu_enclave_id_2) ==> (another_eid == cpu_enclave_id_1);
 
     eid := cpu_enclave_id;
     pc_pa := cpu_addr_map[cpu_pc];
@@ -44,6 +52,14 @@ procedure {:inline 1} MeasurementEnclaveComputation(iter : int)
     
     // operation sync.
     i_eid := uf_load_selector(cpu_pc, pc_op, r0, r1);
+    // if (cpu_enclave_id != another_eid && i_eid == another_eid) {
+    //     i_eid := cpu_enclave_id;
+    // }
+    assume !tap_enclave_metadata_privileged[cpu_enclave_id] ==> i_eid == cpu_enclave_id; 
+    // if (!tap_enclave_metadata_privileged[cpu_enclave_id]) {
+        
+    // }
+    // assume i_eid != cpu_enclave_id_1 && i_eid != cpu_enclave_id_2;
     is_invalid_id :=    ((!tap_enclave_metadata_valid[i_eid]) || 
                          (tap_enclave_metadata_privileged[cpu_enclave_id]  && i_eid != cpu_enclave_id && tap_enclave_metadata_owner_map[i_eid] != cpu_enclave_id) || 
                          (!tap_enclave_metadata_privileged[cpu_enclave_id] && i_eid != cpu_enclave_id));
@@ -104,10 +120,24 @@ procedure {:inline 1} MeasurementEnclaveComputation(iter : int)
     cpu_regs[rd] := uf_cpu_result(cpu_pc, pc_op, l_data, r0, r1);
 }
 // Boogie 2.16.4.0
-//    Error: Parameter to :inline attribute on a function must be Boolean
+//    Parameter to :inline attribute on a function must be Boolean
 function is_measurement_untrusted_op(op : tap_proof_op_t) : bool
 { 
-  op == tap_proof_op_resume || op == tap_proof_op_enter 
+  op == tap_proof_op_resume || 
+  op == tap_proof_op_enter  ||
+  op == tap_proof_op_exit   || 
+  op == tap_proof_op_pause
+}
+
+function is_measurement_privilege_op(op : tap_proof_op_t) : bool
+{
+  op == tap_proof_op_enter      || 
+  op == tap_proof_op_compute    ||
+  op == tap_proof_op_destroy    || 
+  op == tap_proof_op_exit       || 
+  op == tap_proof_op_launch     ||
+  op == tap_proof_op_resume     ||
+  op == tap_proof_op_pause
 }
 
 function is_measurement_enclave_op(op : tap_proof_op_t) : bool
@@ -118,9 +148,10 @@ function is_measurement_enclave_op(op : tap_proof_op_t) : bool
 }
 
 procedure {:inline 1} MeasurementUntrustedOp(
-    /* operation */ op   : tap_proof_op_t, 
-    /* enclave   */ eid  : tap_enclave_id_t,
-    /* args      */ regs : regs_t
+    /* mode      */ mode    : mode_t,
+    /* operation */ op      : tap_proof_op_t, 
+    /* enclave   */ eid     : tap_enclave_id_t,
+    /* args      */ r_regs  : regs_t
 ) 
   returns (status : enclave_op_result_t, current_mode : mode_t)
   modifies cpu_mem;
@@ -139,26 +170,65 @@ procedure {:inline 1} MeasurementUntrustedOp(
   modifies tap_enclave_metadata_paused;
   modifies tap_enclave_metadata_cache_conflict;
 {
+    var regs    : regs_t;
+
     assert (is_measurement_untrusted_op(op));
+    regs := cpu_regs;
     status := enclave_op_success;
+
+    assert (cpu_enclave_id != tap_null_enc_id) ==> 
+        (tap_enclave_metadata_owner_map[cpu_enclave_id] == eid);
+    assert (cpu_enclave_id != tap_null_enc_id) ==> 
+        (tap_enclave_metadata_privileged[tap_enclave_metadata_owner_map[cpu_enclave_id]]);
+
     if (op == tap_proof_op_enter) {
-        cpu_regs := regs;
         call status := enter(eid);
-        assert status == enclave_op_success;
-        current_mode := mode_enclave;
+        cpu_regs := r_regs;
+        
+        assert mode == mode_enclave ==> status == enclave_op_success;
+        if (status == enclave_op_success) {
+            current_mode := mode_enclave;
+        } else {
+            cpu_regs := regs;
+            current_mode := mode_untrusted;
+        }
+
     } else if (op == tap_proof_op_resume) {
         call status := resume(eid);
+        assert mode == mode_enclave ==> status == enclave_op_success;
         if (status == enclave_op_success) {
             current_mode := mode_enclave;
         } else {
             current_mode := mode_untrusted;
         }
+
+    } else if (op == tap_proof_op_exit) {
+        call status := exit();
+        if (status == enclave_op_success) {
+           current_mode := mode_enclave;
+        } else {
+            current_mode := mode_untrusted;
+        }
+        assert mode == mode_enclave ==> status == enclave_op_success;
+
+    } else if (op == tap_proof_op_pause) {
+        call status := pause();
+        if (status == enclave_op_success) {
+            current_mode := mode_enclave;
+        } else {
+            current_mode := mode_untrusted;
+        }
+        assert mode == mode_enclave ==> status == enclave_op_success;
+
     }
+
 }
 
 procedure {:inline 1} MeasurementEnclaveOp(
-    /* operation */ op   : tap_proof_op_t,
-    /* iteration */ iter : int
+    /* mode      */ mode  : mode_t,
+    /* target    */ r_eid : tap_enclave_id_t,
+    /* operation */ op    : tap_proof_op_t,
+    /* iteration */ iter  : int
 ) 
   returns (status : enclave_op_result_t, current_mode : mode_t, vaddr : vaddr_t, word : word_t)
   modifies cpu_mem;
@@ -172,27 +242,108 @@ procedure {:inline 1} MeasurementEnclaveOp(
   modifies tap_enclave_metadata_valid;
   modifies tap_enclave_metadata_addr_map;
   modifies tap_enclave_metadata_addr_valid;
+  modifies tap_enclave_metadata_addr_excl;
   modifies tap_enclave_metadata_entrypoint;
   modifies tap_enclave_metadata_pc;
   modifies tap_enclave_metadata_regs;
   modifies tap_enclave_metadata_paused;
   modifies tap_enclave_metadata_cache_conflict;
+  modifies tap_enclave_metadata_privileged;
+  modifies tap_enclave_metadata_owner_map;
 {
-    assert (is_measurement_enclave_op(op));
+    var regs              : regs_t;
+    var p_regs            : regs_t;
+    var p_container_valid : container_valid_t;
+    var p_container_data  : container_data_t;
+    /* enclave launch structure */
+    var r_addr_valid      : addr_valid_t;
+    var r_addr_map        : addr_map_t;
+    var r_excl_vaddr      : excl_vaddr_t;
+    var r_excl_map        : excl_map_t;
+    var r_entrypoint      : vaddr_t;
+    var r_privileged      : bool;
+
     vaddr := k0_vaddr_t;
     word  := k0_word_t;
-    if (op == tap_proof_op_compute) {
-        call vaddr, word := MeasurementEnclaveComputation(iter);
-        status := enclave_op_success;
-        current_mode := mode_enclave;
-    } else if (op == tap_proof_op_exit) {
-        call status := exit();
-        current_mode := mode_untrusted;
-    } else if (op == tap_proof_op_pause) {
-        call status := pause();
-        current_mode := mode_untrusted;
+    regs  := cpu_regs;
+
+    if (tap_enclave_metadata_privileged[cpu_enclave_id]) {
+        assert is_measurement_privilege_op(op);
+        
+        if (op == tap_proof_op_enter) {
+            call status := enter(r_eid);
+            cpu_regs := p_regs;
+            
+            if (status == enclave_op_success) {
+                current_mode := mode_untrusted;
+            } else {
+                cpu_regs  := regs;
+                current_mode := mode_enclave;
+            }
+            // mode == mode_untrusted means we are in trace_2, sync operation.
+            // sync: all eid's children must be same stage.
+            assert mode == mode_untrusted ==> status == enclave_op_success;
+
+        } else if (op == tap_proof_op_compute) {
+            call vaddr, word := MeasurementEnclaveComputation(iter);
+            status := enclave_op_success;
+            current_mode := mode_enclave;
+
+        } else if (op == tap_proof_op_destroy) {
+            call status := destroy(r_eid);
+            current_mode := mode_enclave;
+
+        } else if (op == tap_proof_op_exit) {
+            call status := exit();
+            assert status == enclave_op_success;
+            current_mode := mode_untrusted;
+
+        } else if (op == tap_proof_op_launch) {
+            assume !tap_enclave_metadata_valid[r_eid];
+            call InitOSMem(p_container_valid, p_container_data);
+            // Apr 6, 2023. add a buildup stage for launch.
+            call r_addr_valid, r_addr_map, r_excl_vaddr, r_excl_map, r_entrypoint, r_privileged := LaunchHavoc(r_eid);
+            call status := launch(r_eid, r_addr_valid, r_addr_map,
+                                r_excl_vaddr, r_excl_map, r_entrypoint, r_privileged);
+            current_mode := mode_enclave;
+
+        } else if (op == tap_proof_op_resume) {
+            call status := resume(r_eid);
+            if (status == enclave_op_success) {
+                current_mode := mode_untrusted;
+            } else {
+                current_mode := mode_enclave;
+            }
+            assert mode == mode_untrusted ==> status == enclave_op_success;
+
+        } else if (op == tap_proof_op_pause) {
+            call status := pause();
+            assert status == enclave_op_success;
+            current_mode := mode_untrusted;
+
+        }
+        
+    } else {
+        assert is_measurement_enclave_op(op);
+
+        if (op == tap_proof_op_compute) {
+            call vaddr, word := MeasurementEnclaveComputation(iter);
+            status := enclave_op_success;
+            current_mode := mode_enclave;
+
+        } else if (op == tap_proof_op_exit) {
+            call status := exit();
+            assert status == enclave_op_success;
+            current_mode := mode_untrusted;
+
+        } else if (op == tap_proof_op_pause) {
+            call status := pause();
+            assert status == enclave_op_success;
+            current_mode := mode_untrusted;
+
+        }
     }
-    assert status == enclave_op_success;
+
 }
 
 //--------------------------------------------------------------------------//
@@ -350,7 +501,76 @@ procedure measurement_proof_part1()
   ensures (forall v : vaddr_t ::
                 tap_enclave_metadata_addr_excl_2[eid_2][v] ==> 
                 (cpu_owner_map_2[tap_enclave_metadata_addr_map_2[eid_2][v]] == eid_2));
-  // extend exclusive memory consistency.
+
+  ensures !tap_enclave_metadata_privileged_1[tap_null_enc_id];
+  ensures !tap_enclave_metadata_privileged_2[tap_null_enc_id];
+  ensures tap_enclave_metadata_privileged_1[eid_1] == tap_enclave_metadata_privileged_2[eid_2];
+  //  privileged relationship: unique PE
+  ensures (e_privileged_1) ==> (forall e : tap_enclave_id_t :: (tap_enclave_metadata_valid_1[e]) ==> 
+          (tap_enclave_metadata_privileged_1[e] <==> e == eid_1));
+  ensures (e_privileged_2) ==> (forall e : tap_enclave_id_t :: (tap_enclave_metadata_valid_2[e]) ==> 
+          (tap_enclave_metadata_privileged_2[e] <==> e == eid_2));
+
+  ensures (!e_privileged_1) ==> (forall e : tap_enclave_id_t :: (tap_enclave_metadata_valid_1[e]) ==> 
+          (!tap_enclave_metadata_privileged_1[e]));
+  ensures (!e_privileged_2) ==> (forall e : tap_enclave_id_t :: (tap_enclave_metadata_valid_2[e]) ==> 
+          (!tap_enclave_metadata_privileged_2[e]));
+
+  // valid guarantee
+  ensures tap_enclave_metadata_valid_1[tap_null_enc_id];
+  ensures tap_enclave_metadata_valid_2[tap_null_enc_id];
+  ensures (forall e : tap_enclave_id_t :: special_enclave_id(e) ==> 
+    !tap_enclave_metadata_valid_1[e]);
+  ensures (forall e : tap_enclave_id_t :: special_enclave_id(e) ==> 
+    !tap_enclave_metadata_valid_2[e]);
+
+  // enclave ownermap relationship: valid enclave's parent must be valid
+  ensures (forall e : tap_enclave_id_t :: tap_enclave_metadata_valid_1[e] ==>
+    (tap_enclave_metadata_valid_1[tap_enclave_metadata_owner_map_1[e]]));
+  ensures (forall e : tap_enclave_id_t :: tap_enclave_metadata_valid_2[e] ==>
+    (tap_enclave_metadata_valid_2[tap_enclave_metadata_owner_map_2[e]]));
+
+  // enclave ownermap relationship: special children
+  ensures tap_enclave_metadata_owner_map_1[eid_1] == tap_null_enc_id;
+  ensures tap_enclave_metadata_owner_map_2[eid_2] == tap_null_enc_id;
+  ensures tap_enclave_metadata_owner_map_1[tap_null_enc_id] == tap_null_enc_id;
+  ensures tap_enclave_metadata_owner_map_2[tap_null_enc_id] == tap_null_enc_id;
+  
+  // enclave ownermap relationship: the maximal parent-tree depth is 2 
+  ensures (forall e : tap_enclave_id_t :: (tap_enclave_metadata_valid_1[e]) ==> 
+    (tap_enclave_metadata_owner_map_1[tap_enclave_metadata_owner_map_1[e]] == tap_null_enc_id));
+  ensures (forall e : tap_enclave_id_t :: (tap_enclave_metadata_valid_2[e]) ==> 
+    (tap_enclave_metadata_owner_map_2[tap_enclave_metadata_owner_map_2[e]] == tap_null_enc_id));
+  
+  // if the mode_untrusted is from PE's children enclave, then the 2 traces is in **one** children enclave of this PE.
+  ensures ((tap_enclave_metadata_owner_map_1[cpu_enclave_id_1] == eid_1) ==> 
+    (tap_enclave_metadata_valid_2[cpu_enclave_id_2]));
+  ensures ((tap_enclave_metadata_owner_map_1[cpu_enclave_id_1] == eid_1) ==>
+    (tap_enclave_metadata_owner_map_2[cpu_enclave_id_2] == eid_2));
+  
+  // enclave ownermap relationship: enclave with chidren must be privileged 
+  ensures (forall e : tap_enclave_id_t :: 
+    (tap_enclave_metadata_valid_1[e] && tap_enclave_metadata_owner_map_1[e] != tap_null_enc_id) ==> 
+      (tap_enclave_metadata_privileged_1[tap_enclave_metadata_owner_map_1[e]]));
+  ensures (forall e : tap_enclave_id_t :: 
+    (tap_enclave_metadata_valid_2[e] && tap_enclave_metadata_owner_map_2[e] != tap_null_enc_id) ==> 
+      (tap_enclave_metadata_privileged_2[tap_enclave_metadata_owner_map_2[e]]));
+
+  // extend exclusive memory consistency and structure rules. Apr 14, 2023.
+  ensures (forall e : tap_enclave_id_t, v : vaddr_t :: 
+    (tap_enclave_metadata_valid_1[e] && (tap_enclave_metadata_privileged_1[e] || tap_enclave_metadata_privileged_1[tap_enclave_metadata_owner_map_1[e]]) ==> 
+        (tap_enclave_metadata_addr_excl_1[e][v] <==> cpu_owner_map_1[tap_enclave_metadata_addr_map_1[e][v]] == e)));
+  ensures (forall e : tap_enclave_id_t, v : vaddr_t :: 
+    (tap_enclave_metadata_valid_2[e] && (tap_enclave_metadata_privileged_2[e] || tap_enclave_metadata_privileged_2[tap_enclave_metadata_owner_map_2[e]]) ==> 
+        (tap_enclave_metadata_addr_excl_2[e][v] <==> cpu_owner_map_2[tap_enclave_metadata_addr_map_2[e][v]] == e)));
+  // PE sync. the PE's structure must be same.
+  ensures (forall e : tap_enclave_id_t :: 
+        (tap_enclave_metadata_valid_1[e] && tap_enclave_metadata_owner_map_1[e] == eid_1) <==> 
+            (tap_enclave_metadata_valid_2[e] && tap_enclave_metadata_owner_map_2[e] == eid_2));
+  // PE sync. the two (PE) enclave's children pause state must be same. 
+  ensures (forall e : tap_enclave_id_t :: 
+        (tap_enclave_metadata_valid_1[e] && tap_enclave_metadata_owner_map_1[e] == eid_1) ==> 
+            (tap_enclave_metadata_paused_1[e] == tap_enclave_metadata_paused_2[e]));
 
   //----------------------------------------------------------------------//
   // invariants about the states of the CPUs.                             //
@@ -439,7 +659,8 @@ procedure measurement_proof_part2
   /* addr_map   */  e_addr_map_1, e_addr_map_2     : addr_map_t,
   /* excl vaddr */  e_addr_excl_1, e_addr_excl_2   : excl_vaddr_t,
   /* excl       */  e_excl_map_1, e_excl_map_2     : excl_map_t,
-  /* entrypoint */  e_entrypoint_1, e_entrypoint_2 : vaddr_t
+  /* entrypoint */  e_entrypoint_1, e_entrypoint_2 : vaddr_t,
+  /* privileged */  e_privileged_1, e_privileged_2 : bool
 )
   
   modifies cpu_mem;
@@ -509,6 +730,7 @@ procedure measurement_proof_part2
                                     cpu_mem_1, cpu_mem_2, v));
   requires (forall ri : regindex_t :: valid_regindex(ri) ==> (cpu_regs_1[ri] == cpu_regs_2[ri]));
   requires (e_entrypoint_1 == e_entrypoint_2);
+  requires (e_privileged_1 == e_privileged_2);
   requires  (forall pa : wap_addr_t, e : tap_enclave_id_t ::
               (valid_enclave_id(e) && !tap_enclave_metadata_valid_1[e]) ==> 
                   (cpu_owner_map_1[pa] != e));
@@ -581,7 +803,72 @@ procedure measurement_proof_part2
             cpu_enclave_id_2 == tap_null_enc_id);
   requires (tap_addr_perm_x(cpu_addr_valid_1[cpu_pc_1]) && 
             tap_addr_perm_x(cpu_addr_valid_2[cpu_pc_2]));
+  //----------------------------------------------------------------------//
+  // invariants about PE-related structure rules                          //
+  //----------------------------------------------------------------------//
+  requires !tap_enclave_metadata_privileged_1[tap_null_enc_id];
+  requires !tap_enclave_metadata_privileged_2[tap_null_enc_id];
+  requires  tap_enclave_metadata_privileged_1[eid_1] == tap_enclave_metadata_privileged_2[eid_2];
+  //  privileged relationship: unique PE
+  requires (e_privileged_1) ==> (forall e : tap_enclave_id_t :: (tap_enclave_metadata_valid_1[e]) ==> 
+            (tap_enclave_metadata_privileged_1[e] <==> e == eid_1));
+  requires (e_privileged_2) ==> (forall e : tap_enclave_id_t :: (tap_enclave_metadata_valid_2[e]) ==> 
+            (tap_enclave_metadata_privileged_2[e] <==> e == eid_2));
+  requires (!e_privileged_1) ==> (forall e : tap_enclave_id_t :: (tap_enclave_metadata_valid_1[e]) ==> 
+            (!tap_enclave_metadata_privileged_1[e]));
+  requires (!e_privileged_2) ==> (forall e : tap_enclave_id_t :: (tap_enclave_metadata_valid_2[e]) ==> 
+            (!tap_enclave_metadata_privileged_2[e]));
+  // valid guarantee
+  requires tap_enclave_metadata_valid_1[tap_null_enc_id];
+  requires tap_enclave_metadata_valid_2[tap_null_enc_id];
+  requires (forall e : tap_enclave_id_t :: special_enclave_id(e) ==> 
+            !tap_enclave_metadata_valid_1[e]);
+  requires (forall e : tap_enclave_id_t :: special_enclave_id(e) ==> 
+            !tap_enclave_metadata_valid_2[e]);
+  // enclave ownermap relationship: valid enclave's parent must be valid
+  requires (forall e : tap_enclave_id_t :: tap_enclave_metadata_valid_1[e] ==>
+          (tap_enclave_metadata_valid_1[tap_enclave_metadata_owner_map_1[e]]));
+  requires (forall e : tap_enclave_id_t :: tap_enclave_metadata_valid_2[e] ==>
+          (tap_enclave_metadata_valid_2[tap_enclave_metadata_owner_map_2[e]]));
+  // enclave ownermap relationship: special children
+  requires tap_enclave_metadata_owner_map_1[eid_1] == tap_null_enc_id;
+  requires tap_enclave_metadata_owner_map_2[eid_2] == tap_null_enc_id;
+  requires tap_enclave_metadata_owner_map_1[tap_null_enc_id] == tap_null_enc_id;
+  requires tap_enclave_metadata_owner_map_2[tap_null_enc_id] == tap_null_enc_id;
+  // enclave ownermap relationship: the maximal parent-tree depth is 2 
+  requires (forall e : tap_enclave_id_t :: (tap_enclave_metadata_valid_1[e]) ==> 
+          (tap_enclave_metadata_owner_map_1[tap_enclave_metadata_owner_map_1[e]] == tap_null_enc_id));
+  requires (forall e : tap_enclave_id_t :: (tap_enclave_metadata_valid_2[e]) ==> 
+          (tap_enclave_metadata_owner_map_2[tap_enclave_metadata_owner_map_2[e]] == tap_null_enc_id));
+  // if the mode_untrusted is from PE's children enclave, then the 2 traces is in **one** children enclave of this PE.
+  requires ((tap_enclave_metadata_owner_map_1[cpu_enclave_id_1] == eid_1) ==> 
+          (tap_enclave_metadata_valid_2[cpu_enclave_id_2]));
+  requires ((tap_enclave_metadata_owner_map_1[cpu_enclave_id_1] == eid_1) ==>
+          (tap_enclave_metadata_owner_map_2[cpu_enclave_id_2] == eid_2));
+  // enclave ownermap relationship: enclave with chidren must be privileged 
+  requires (forall e : tap_enclave_id_t :: 
+          (tap_enclave_metadata_valid_1[e] && tap_enclave_metadata_owner_map_1[e] != tap_null_enc_id) ==> 
+                (tap_enclave_metadata_privileged_1[tap_enclave_metadata_owner_map_1[e]]));
+  requires (forall e : tap_enclave_id_t :: 
+          (tap_enclave_metadata_valid_2[e] && tap_enclave_metadata_owner_map_2[e] != tap_null_enc_id) ==> 
+                (tap_enclave_metadata_privileged_2[tap_enclave_metadata_owner_map_2[e]]));
+  // extend exclusive memory consistency and structure rules. Apr 14, 2023.
+  requires (forall e : tap_enclave_id_t, v : vaddr_t :: 
+          (tap_enclave_metadata_valid_1[e] && (tap_enclave_metadata_privileged_1[e] || tap_enclave_metadata_privileged_1[tap_enclave_metadata_owner_map_1[e]]) ==> 
+                (tap_enclave_metadata_addr_excl_1[e][v] <==> cpu_owner_map_1[tap_enclave_metadata_addr_map_1[e][v]] == e)));
+  requires (forall e : tap_enclave_id_t, v : vaddr_t :: 
+          (tap_enclave_metadata_valid_2[e] && (tap_enclave_metadata_privileged_2[e] || tap_enclave_metadata_privileged_2[tap_enclave_metadata_owner_map_2[e]]) ==> 
+                (tap_enclave_metadata_addr_excl_2[e][v] <==> cpu_owner_map_2[tap_enclave_metadata_addr_map_2[e][v]] == e)));
+  // PE sync. the PE's structure must be same.
+  requires (forall e : tap_enclave_id_t :: 
+          (tap_enclave_metadata_valid_1[e] && tap_enclave_metadata_owner_map_1[e] == eid_1) <==> 
+                (tap_enclave_metadata_valid_2[e] && tap_enclave_metadata_owner_map_2[e] == eid_2));
+  // PE sync. the two (PE) enclave's children pause state must be same. 
+  requires (forall e : tap_enclave_id_t :: 
+          (tap_enclave_metadata_valid_1[e] && tap_enclave_metadata_owner_map_1[e] == eid_1) ==> 
+                (tap_enclave_metadata_paused_1[e] == tap_enclave_metadata_paused_2[e]));
 {
+  var r_eid                                        : tap_enclave_id_t;
   var status, status_1, status_2                   : enclave_op_result_t;
   var e_container_data_1, e_container_data_2       : container_data_t;
   var enclave_dead_1, enclave_dead_2               : bool;
@@ -593,7 +880,7 @@ procedure measurement_proof_part2
   var memp_1, memp_2                               : mem_t;
   var word_1, word_2                               : word_t;
   var proof_op                                     : tap_proof_op_t;
-  var regs                                         : regs_t;
+  var regs, r_regs                                 : regs_t;
   var shared_vaddr_map                             : shared_vaddr_map_t;
   var current_mode                                 : mode_t;
   var current_mode_1, current_mode_2               : mode_t;
@@ -604,12 +891,85 @@ procedure measurement_proof_part2
     //----------------------------------------------------------------------//
     // global TAP invariants.                                               //
     //----------------------------------------------------------------------//
+    
+    // privilege relationship: OS & eid
+    invariant !tap_enclave_metadata_privileged_1[tap_null_enc_id];
+    invariant !tap_enclave_metadata_privileged_2[tap_null_enc_id];
+    invariant tap_enclave_metadata_privileged_1[eid_1] == tap_enclave_metadata_privileged_2[eid_2];
+
+    //  privileged relationship: unique PE
+    invariant (e_privileged_1) ==> (forall e : tap_enclave_id_t :: (tap_enclave_metadata_valid_1[e]) ==> 
+            (tap_enclave_metadata_privileged_1[e] <==> e == eid_1));
+    invariant (e_privileged_2) ==> (forall e : tap_enclave_id_t :: (tap_enclave_metadata_valid_2[e]) ==> 
+            (tap_enclave_metadata_privileged_2[e] <==> e == eid_2));
+
+    invariant (!e_privileged_1) ==> (forall e : tap_enclave_id_t :: (tap_enclave_metadata_valid_1[e]) ==> 
+            (!tap_enclave_metadata_privileged_1[e]));
+    invariant (!e_privileged_2) ==> (forall e : tap_enclave_id_t :: (tap_enclave_metadata_valid_2[e]) ==> 
+            (!tap_enclave_metadata_privileged_2[e]));
+
+    // valid guarantee
+    invariant tap_enclave_metadata_valid_1[tap_null_enc_id];
+    invariant tap_enclave_metadata_valid_2[tap_null_enc_id];
+    invariant (forall e : tap_enclave_id_t :: special_enclave_id(e) ==> 
+        !tap_enclave_metadata_valid_1[e]);
+    invariant (forall e : tap_enclave_id_t :: special_enclave_id(e) ==> 
+        !tap_enclave_metadata_valid_2[e]);
+
+    // enclave ownermap relationship: valid enclave's parent must be valid
+    invariant (forall e : tap_enclave_id_t :: tap_enclave_metadata_valid_1[e] ==>
+        (tap_enclave_metadata_valid_1[tap_enclave_metadata_owner_map_1[e]]));
+    invariant (forall e : tap_enclave_id_t :: tap_enclave_metadata_valid_2[e] ==>
+        (tap_enclave_metadata_valid_2[tap_enclave_metadata_owner_map_2[e]]));
+
+    // enclave ownermap relationship: special children
+    invariant tap_enclave_metadata_owner_map_1[eid_1] == tap_null_enc_id;
+    invariant tap_enclave_metadata_owner_map_2[eid_2] == tap_null_enc_id;
+    invariant tap_enclave_metadata_owner_map_1[tap_null_enc_id] == tap_null_enc_id;
+    invariant tap_enclave_metadata_owner_map_2[tap_null_enc_id] == tap_null_enc_id;
+    
+    // enclave ownermap relationship: the maximal parent-tree depth is 2 
+    invariant (forall e : tap_enclave_id_t :: (tap_enclave_metadata_valid_1[e]) ==> 
+        (tap_enclave_metadata_owner_map_1[tap_enclave_metadata_owner_map_1[e]] == tap_null_enc_id));
+    invariant (forall e : tap_enclave_id_t :: (tap_enclave_metadata_valid_2[e]) ==> 
+        (tap_enclave_metadata_owner_map_2[tap_enclave_metadata_owner_map_2[e]] == tap_null_enc_id));
+    
+    // if the mode_untrusted is from PE's children enclave, then the 2 traces is in **one** children enclave of this PE.
+    invariant ((tap_enclave_metadata_owner_map_1[cpu_enclave_id_1] == eid_1) ==> 
+        (tap_enclave_metadata_valid_2[cpu_enclave_id_2]));
+    invariant ((tap_enclave_metadata_owner_map_1[cpu_enclave_id_1] == eid_1) ==>
+        (tap_enclave_metadata_owner_map_2[cpu_enclave_id_2] == eid_2));
+    
+    // enclave ownermap relationship: enclave with chidren must be privileged 
+    invariant (forall e : tap_enclave_id_t :: 
+        (tap_enclave_metadata_valid_1[e] && tap_enclave_metadata_owner_map_1[e] != tap_null_enc_id) ==> 
+          (tap_enclave_metadata_privileged_1[tap_enclave_metadata_owner_map_1[e]]));
+    invariant (forall e : tap_enclave_id_t :: 
+        (tap_enclave_metadata_valid_2[e] && tap_enclave_metadata_owner_map_2[e] != tap_null_enc_id) ==> 
+          (tap_enclave_metadata_privileged_2[tap_enclave_metadata_owner_map_2[e]]));
+
+    // pa ownermap wouldn't point to invalid enclave.
     invariant  (forall pa : wap_addr_t, e : tap_enclave_id_t ::
                 (valid_enclave_id(e) && !tap_enclave_metadata_valid_1[e]) ==> 
                     (cpu_owner_map_1[pa] != e));
     invariant  (forall pa : wap_addr_t, e : tap_enclave_id_t ::
                 (valid_enclave_id(e) && !tap_enclave_metadata_valid_2[e]) ==> 
                     (cpu_owner_map_2[pa] != e));
+
+    // extend exclusive memory consistency and structure rules. Apr 14, 2023.
+    invariant (forall e : tap_enclave_id_t, v : vaddr_t :: 
+        (tap_enclave_metadata_valid_1[e] && (tap_enclave_metadata_privileged_1[e] || tap_enclave_metadata_privileged_1[tap_enclave_metadata_owner_map_1[e]]) ==> 
+            (tap_enclave_metadata_addr_excl_1[e][v] <==> cpu_owner_map_1[tap_enclave_metadata_addr_map_1[e][v]] == e)));
+    invariant (forall e : tap_enclave_id_t, v : vaddr_t :: 
+        (tap_enclave_metadata_valid_2[e] && (tap_enclave_metadata_privileged_2[e] || tap_enclave_metadata_privileged_2[tap_enclave_metadata_owner_map_2[e]]) ==> 
+            (tap_enclave_metadata_addr_excl_2[e][v] <==> cpu_owner_map_2[tap_enclave_metadata_addr_map_2[e][v]] == e)));
+    invariant (forall v : vaddr_t :: 
+        (!enclave_dead_1 && (tap_enclave_metadata_privileged_1[cpu_enclave_id_1] || tap_enclave_metadata_privileged_1[tap_enclave_metadata_owner_map_1[cpu_enclave_id_1]])) ==> 
+            (tap_enclave_metadata_addr_excl_1[cpu_enclave_id_1][v] <==> cpu_owner_map_1[cpu_addr_map_1[v]] == cpu_enclave_id_1));
+    invariant (forall v : vaddr_t :: 
+        (!enclave_dead_2 && (tap_enclave_metadata_privileged_2[cpu_enclave_id_2] || tap_enclave_metadata_privileged_2[tap_enclave_metadata_owner_map_2[cpu_enclave_id_2]])) ==> 
+            (tap_enclave_metadata_addr_excl_2[cpu_enclave_id_2][v] <==> cpu_owner_map_2[cpu_addr_map_2[v]] == cpu_enclave_id_2));
+
     // eid is valid.
     invariant (valid_enclave_id(eid_1) && valid_enclave_id(eid_2));
     invariant (tap_enclave_metadata_valid_1[eid_1] && tap_enclave_metadata_valid_2[eid_2]);
@@ -651,8 +1011,30 @@ procedure measurement_proof_part2
     //----------------------------------------------------------------------//
     // invariants about the states of the CPUs.                             //
     //----------------------------------------------------------------------//
-    invariant (current_mode == mode_untrusted) ==>
-                (cpu_enclave_id_1 == tap_null_enc_id && cpu_enclave_id_2 == tap_null_enc_id);
+
+    // invariants about state sync between 2 traces.
+    // These properties may need extension/modification for multiple PE environment.
+    // OS/NE sync. (stronger than Integrity's)
+    invariant (current_mode == mode_untrusted) ==> 
+                  (cpu_enclave_id_1 == cpu_enclave_id_2);
+    invariant (current_mode == mode_untrusted) ==> 
+                  (cpu_enclave_id_1 == tap_null_enc_id) || 
+                  (tap_enclave_metadata_owner_map_1[cpu_enclave_id_1] == eid_1);
+    // PE sync. the PE's structure must be same.
+    invariant (forall e : tap_enclave_id_t :: 
+        (tap_enclave_metadata_valid_1[e] && tap_enclave_metadata_owner_map_1[e] == eid_1) <==> 
+            (tap_enclave_metadata_valid_2[e] && tap_enclave_metadata_owner_map_2[e] == eid_2));
+
+    // PE sync. the two (PE) enclave's children pause state must be same. 
+    // Apr 4, 2023.
+    invariant (!enclave_dead_1 && !enclave_dead_2) ==>
+                (forall e : tap_enclave_id_t :: 
+                    (tap_enclave_metadata_valid_1[e] && tap_enclave_metadata_owner_map_1[e] == eid_1) ==> 
+                        tap_enclave_metadata_paused_1[e] == tap_enclave_metadata_paused_2[e]);
+    
+    invariant (current_mode == mode_untrusted) ==> tap_enclave_metadata_valid_1[cpu_enclave_id_1];
+    invariant (current_mode == mode_untrusted) ==> tap_enclave_metadata_valid_2[cpu_enclave_id_2];
+
     invariant (current_mode == mode_enclave) ==> 
                 (cpu_enclave_id_1 == eid_1 && cpu_enclave_id_2 == eid_2);
     invariant (current_mode == mode_enclave) ==>
@@ -708,29 +1090,35 @@ procedure measurement_proof_part2
                     (tap_enclave_metadata_addr_map_2[eid_2] == cpu_addr_map_2);
     invariant (current_mode == mode_enclave || current_mode == mode_untrusted);
   {
-    havoc proof_op;
-    havoc regs;
+    havoc r_eid, proof_op, r_regs;
     if (current_mode == mode_untrusted) {
-      assume (is_measurement_untrusted_op(proof_op));
-      // assume (proof_op != tap_proof_op_resume);
+      assume false;
+      assume is_measurement_untrusted_op(proof_op);
       call RestoreContext_1();
-      call status_1, current_mode_1 := MeasurementUntrustedOp(proof_op, eid_1, regs);
+      call status_1, current_mode_1 := MeasurementUntrustedOp(current_mode, proof_op, eid_1, r_regs);
       call SaveContext_1();
 
       call RestoreContext_2();
-      call status_2, current_mode_2 := MeasurementUntrustedOp(proof_op, eid_2, regs);
+      call status_2, current_mode_2 := MeasurementUntrustedOp(current_mode, proof_op, eid_2, r_regs);
       call SaveContext_2();
-    } else if (current_mode == mode_enclave) {
-      havoc iter;
 
-      assume (is_measurement_enclave_op(proof_op));
-      // assume (proof_op != tap_proof_op_pause);
+    } else if (current_mode == mode_enclave) {
+      // assume false;
+      assume !e_privileged_1;
+      havoc iter;
+      if (e_privileged_1) {
+        assume is_measurement_privilege_op(proof_op);
+      } else {
+        assume is_measurement_enclave_op(proof_op);
+      }
+      assume r_eid != eid_1 && r_eid != eid_2;
+      
       call RestoreContext_1();
-      call status_1, current_mode_1, vaddr_1, word_1 := MeasurementEnclaveOp(proof_op, iter);
+      call status_1, current_mode_1, vaddr_1, word_1 := MeasurementEnclaveOp(current_mode, r_eid, proof_op, iter);
       call SaveContext_1();
 
       call RestoreContext_2();
-      call status_2, current_mode_2, vaddr_2, word_2 := MeasurementEnclaveOp(proof_op, iter);
+      call status_2, current_mode_2, vaddr_2, word_2 := MeasurementEnclaveOp(current_mode, r_eid, proof_op, iter);
       call SaveContext_2();
 
       assert vaddr_1 == vaddr_2;
@@ -818,11 +1206,12 @@ procedure measurement_proof()
        e_privileged_1, e_privileged_2,
        current_mode                     := measurement_proof_part1();
   // proof stage 2.
-  // call measurement_proof_part2(
-  //        eid_1, eid_2,
-  //        e_addr_valid_1, e_addr_valid_2,
-  //        e_addr_map_1, e_addr_map_2,
-  //        e_excl_vaddr_1, e_excl_vaddr_2,
-  //        e_excl_map_1, e_excl_map_2,
-  //        e_entrypoint_1, e_entrypoint_2);
+  call measurement_proof_part2(
+         eid_1, eid_2,
+         e_addr_valid_1, e_addr_valid_2,
+         e_addr_map_1, e_addr_map_2,
+         e_excl_vaddr_1, e_excl_vaddr_2,
+         e_excl_map_1, e_excl_map_2,
+         e_entrypoint_1, e_entrypoint_2,
+         e_privileged_1, e_privileged_2);
 }
