AbstractPlatform/Types.bpl
@@ -193,7 +193,6 @@ function tap_proof_op_valid_in_privileged (o : tap_proof_op_t) : bool
     o == tap_proof_op_enter   ||
     o == tap_proof_op_compute   ||
     o == tap_proof_op_destroy || 
-    o == tap_proof_op_enter     ||
     o == tap_proof_op_exit     ||
     o == tap_proof_op_launch   ||
     o == tap_proof_op_resume  ||   
